Foundation/Modal/Kripke/Hilbert/K4Point1.lean
@@ -1,0 +1,34 @@
+import Foundation.Modal.Kripke.Hilbert.K4
+import Foundation.Modal.Kripke.AxiomM
+
+namespace LO.Modal
+
+open Kripke
+open Geachean
+
+instance : TransitiveMcKinseyanFrameClass.DefinedBy Hilbert.K4Point1.axioms :=
+  FrameClass.definedBy_with_axiomK $ TransitiveMcKinseyanFrameClass.DefinedByFourAndM
+
+namespace Hilbert.K4Point1
+
+instance Kripke.sound : Sound (Hilbert.K4Point1) (Kripke.TransitiveMcKinseyanFrameClass) := inferInstance
+
+instance Kripke.consistent : Entailment.Consistent (Hilbert.K4Point1) :=
+  Kripke.Hilbert.consistent_of_FrameClass Kripke.TransitiveMcKinseyanFrameClass
+
+open
+  Kripke
+  MaximalConsistentSet
+in
+instance Kripke.canonical : Canonical (Hilbert.K4Point1) TransitiveMcKinseyanFrameClass := by
+  have hK4 := canonicalFrame.multigeachean_of_provable_geach (G := {⟨0, 2, 1, 0⟩}) (𝓢 := Hilbert.K4Point1) (by simp);
+  constructor;
+  refine ⟨?_, ?_⟩;
+  . simpa [transitive_def] using @hK4 (⟨0, 2, 1, 0⟩) $ by tauto;
+  . sorry;
+
+instance Kripke.complete : Complete (Hilbert.K4Point1) TransitiveMcKinseyanFrameClass := inferInstance
+
+end Hilbert.K4Point1
+
+end LO.Modal
