Foundation/Modal/Kripke/Hilbert/S4Point1.lean
@@ -1,0 +1,34 @@
+import Foundation.Modal.Kripke.Hilbert.KT
+import Foundation.Modal.Kripke.Hilbert.K4Point1
+
+namespace LO.Modal
+
+open Kripke
+open Geachean
+
+abbrev Kripke.ReflexiveTransitiveMcKinseyanFrameClass : FrameClass := { F | Reflexive F ∧ Transitive F ∧ McKinseyan F }
+
+instance : ReflexiveTransitiveMcKinseyanFrameClass.DefinedBy Hilbert.S4Point1.axioms := by
+  rw [
+    (show ReflexiveTransitiveMcKinseyanFrameClass = TransitiveMcKinseyanFrameClass ∩ ReflexiveFrameClass by aesop),
+    (show Hilbert.S4Point1.axioms = Hilbert.K4Point1.axioms ∪ {Axioms.T (.atom 0)} by aesop)
+  ];
+  exact FrameClass.definedBy_inter Kripke.TransitiveMcKinseyanFrameClass (Hilbert.K4Point1.axioms) ReflexiveFrameClass {Axioms.T (.atom 0)};
+
+instance : Kripke.ReflexiveTransitiveMcKinseyanFrameClass.IsNonempty := by
+  use ⟨Unit, λ _ _ => True⟩;
+  simp [Reflexive, Transitive, McKinseyan];
+
+
+namespace Hilbert.S4Point1
+
+instance Kripke.sound : Sound (Hilbert.S4Point1) (Kripke.ReflexiveTransitiveMcKinseyanFrameClass) := inferInstance
+
+instance Kripke.consistent : Entailment.Consistent (Hilbert.S4Point1) :=
+  Kripke.Hilbert.consistent_of_FrameClass Kripke.ReflexiveTransitiveMcKinseyanFrameClass
+
+instance Kripke.complete : Complete (Hilbert.S4Point1) ReflexiveTransitiveMcKinseyanFrameClass := by sorry;
+
+end Hilbert.S4Point1
+
+end LO.Modal
